p256: rm extra lemmas in Hacl.Spec.P256.Math

code/ecdsap256/Hacl.Spec.P256.Math.fst
@@ -1,7 +1,7 @@
 module Hacl.Spec.P256.Math
 
 open FStar.Mul
-open Spec.P256
+module S = Spec.P256
 
 #set-options "--z3rlimit 50 --fuel 0 --ifuel 0"
 
@@ -19,78 +19,59 @@ let sub_mod n a b =
   Math.Lemmas.mod_add_both (a - b) 0 b n
 
 
-val lemma_modular_multiplication_pow256: a:int -> b:int -> Lemma
-  (requires a * pow2 256 % prime = b * pow2 256 % prime)
-  (ensures  a % prime == b % prime)
+val lemma_mod_mul_pow256_prime: a:int -> b:int -> Lemma
+  (requires a * pow2 256 % S.prime = b * pow2 256 % S.prime)
+  (ensures  a % S.prime == b % S.prime)
 
-let lemma_modular_multiplication_pow256 a b =
-  mod_sub prime (a * pow2 256) (b * pow2 256);
-  assert (pow2 256 * (a - b) % prime = 0);
+let lemma_mod_mul_pow256_prime a b =
+  mod_sub S.prime (a * pow2 256) (b * pow2 256);
+  assert (pow2 256 * (a - b) % S.prime = 0);
   let r = 26959946654596436323893653559348051827142583427821597254581997273087 in
   let s = -26959946648319334592891477706824406424704094582978235142356758167551 in
-  assert_norm (r * prime + s * pow2 256 = 1);
-  FStar.Math.Euclid.euclid prime (pow2 256) (a - b) r s;
-  assert ((a - b) % prime = 0);
-  sub_mod prime a b;
-  assert (a % prime = b % prime)
+  assert_norm (r * S.prime + s * pow2 256 = 1);
+  FStar.Math.Euclid.euclid S.prime (pow2 256) (a - b) r s;
+  assert ((a - b) % S.prime = 0);
+  sub_mod S.prime a b;
+  assert (a % S.prime = b % S.prime)
 
 
-val lemma_modular_multiplication_pow256_order: a:int -> b:int -> Lemma
-  (requires a * pow2 256 % order = b * pow2 256 % order)
-  (ensures  a % order == b % order)
+val lemma_mod_mul_pow256_order: a:int -> b:int -> Lemma
+  (requires a * pow2 256 % S.order = b * pow2 256 % S.order)
+  (ensures  a % S.order == b % S.order)
 
-let lemma_modular_multiplication_pow256_order a b =
-  mod_sub order (a * pow2 256) (b * pow2 256);
-  assert (pow2 256 * (a - b) % order = 0);
+let lemma_mod_mul_pow256_order a b =
+  mod_sub S.order (a * pow2 256) (b * pow2 256);
+  assert (pow2 256 * (a - b) % S.order = 0);
   let r = -43790243024438006127650828685417305984841428635278707415088219106730833919055 in
   let s = 43790243014242295660885426880012836369732278457577312309071968676491870960761 in
-  assert_norm (r * order + s * pow2 256 = 1);
-  FStar.Math.Euclid.euclid order (pow2 256) (a - b) r s;
-  assert ((a - b) % order = 0);
-  sub_mod order a b;
-  assert (a % order = b % order)
+  assert_norm (r * S.order + s * pow2 256 = 1);
+  FStar.Math.Euclid.euclid S.order (pow2 256) (a - b) r s;
+  assert ((a - b) % S.order = 0);
+  sub_mod S.order a b;
+  assert (a % S.order = b % S.order)
 
 
-val lemma_modular_multiplication_p256_2_left:
-  a:nat{a < prime} -> b:nat{b < prime} -> Lemma
-  (requires a * pow2 256 % prime = b * pow2 256 % prime)
-  (ensures  a == b)
-
-let lemma_modular_multiplication_p256_2_left a b =
-  lemma_modular_multiplication_pow256 a b;
-  FStar.Math.Lemmas.modulo_lemma a prime;
-  FStar.Math.Lemmas.modulo_lemma b prime
-
-
-// used in Hacl.Impl.P256.Point
-val lemma_modular_multiplication_p256_2: a: nat{a < prime} -> b: nat{b < prime} ->
-  Lemma (a * pow2 256 % prime = b * pow2 256 % prime <==> a == b)
-
-let lemma_modular_multiplication_p256_2 a b =
-  Classical.move_requires_2 lemma_modular_multiplication_p256_2_left a b
-
-
-val lemma_multiplication_not_mod_prime_left: a:nat{a < prime} -> Lemma
-  (requires a * (modp_inv2_prime (pow2 256) prime) % prime == 0)
+val lemma_multiplication_not_mod_prime_left: a:S.felem -> Lemma
+  (requires a * (S.modp_inv2_prime (pow2 256) S.prime) % S.prime == 0)
   (ensures a == 0)
 
 let lemma_multiplication_not_mod_prime_left a =
-  let b = modp_inv2_prime (pow2 256) prime in
-  Math.Lemmas.lemma_mod_mul_distr_r a b prime;
-  assert (a * b % prime == a * (b % prime) % prime);
+  let b = S.modp_inv2_prime (pow2 256) S.prime in
+  Math.Lemmas.lemma_mod_mul_distr_r a b S.prime;
+  assert (a * b % S.prime == a * (b % S.prime) % S.prime);
   let r = -26959946654596436328278158470660195847911760999080590586820792680449 in
   let s = 26959946660873538059280334323183841250350249843923952699046031785985 in
-  assert_norm (r * prime + s * b == 1);
+  assert_norm (r * S.prime + s * b == 1);
   Math.Lemmas.swap_mul a b;
-  assert (b * a % prime == 0);
-  Math.Euclid.euclid prime b a r s;
-  assert (a % prime == 0);
-  Math.Lemmas.small_mod a prime
+  assert (b * a % S.prime == 0);
+  Math.Euclid.euclid S.prime b a r s;
+  assert (a % S.prime == 0);
+  Math.Lemmas.small_mod a S.prime
 
 
-// used in Hacl.Impl.P256.PointAdd, Hacl.Impl.P256.PointMul, Hacl.Impl.P256.Point
-val lemma_multiplication_not_mod_prime: a:nat{a < prime} ->
-  Lemma (a * (modp_inv2_prime (pow2 256) prime) % prime == 0 <==> a == 0)
+// used in Hacl.Impl.P256.PointAdd, Hacl.Impl.P256.Point
+val lemma_multiplication_not_mod_prime: a:S.felem ->
+  Lemma (a * (S.modp_inv2_prime (pow2 256) S.prime) % S.prime == 0 <==> a == 0)
 
 let lemma_multiplication_not_mod_prime a =
   Classical.move_requires lemma_multiplication_not_mod_prime_left a
