code/ecdsap256/Hacl.Impl.P256.Scalar.fst
@@ -183,7 +183,7 @@ let qmont_R_inv_is_bn_mont_d () =
   assert (qmont_R_inv * pow2 256 % S.order = 1);
 
   assert (qmont_R_inv * pow2 256 % S.order = d * pow2 256 % S.order);
-  Hacl.Spec.P256.Math.lemma_modular_multiplication_pow256_order qmont_R_inv d;
+  Hacl.Spec.P256.Math.lemma_mod_mul_pow256_order qmont_R_inv d;
   assert (qmont_R_inv % S.order == d % S.order);
   Math.Lemmas.modulo_lemma qmont_R_inv S.order;
   assert (qmont_R_inv == d % S.order)
